Update ARMv6 backend proof to support arm6_backend_correct_alt.
ASM has also been tweaked with regard to code_alignment.

targets/asmLib.sig
@@ -6,6 +6,9 @@ sig
    val byte_eq_tac: Tactical.tactic
    val dest_bytes_in_memory:
       Term.term -> Term.term * Term.term * Term.term * Term.term
+   val env_tac:
+      (Term.term * Term.term -> Term.term * Tactic.tactic) -> Tactic.tactic
+   val find_env: Term.term -> (Term.term * Term.term) option
    val mk_bytes_in_memory:
       Term.term * Term.term * Term.term * Term.term -> Term.term
    val strip_bytes_in_memory: Term.term -> Term.term list option
